Core/Ty/Substitution.lean
@@ -1,4 +1,5 @@
 import Core.Vec
+import Core.Util
 import Core.Ty.Definition
 
 open Lilac
@@ -7,16 +8,16 @@ open LeanSubst
 namespace Core
 
 @[coe]
-def Ty.from_action : Subst.Action Ty -> Ty
+def Ty.from_action : Action Ty -> Ty
 | .re y => t#y
 | .su t => t
 
 @[simp]
-theorem Ty.from_action_id {n} : from_action (+0 n) = t#n := by
+theorem Ty.from_action_id {n} : from_action (+0σ.act n) = t#n := by
   simp [from_action, Subst.id]
 
 @[simp]
-theorem Ty.from_action_succ {n} : from_action (+1 n) = t#(n + 1) := by
+theorem Ty.from_action_succ {n} : from_action (+1σ.act n) = t#(n + 1) := by
   simp [from_action, Subst.succ]
 
 @[simp]
@@ -25,54 +26,54 @@ theorem Ty.from_acton_re {n} : from_action (re n) = t#n := by simp [from_action]
 @[simp]
 theorem Ty.from_action_su {t} : from_action (su t) = t := by simp [from_action]
 
-instance : Coe (Subst.Action Ty) Ty where
+instance : Coe (Action Ty) Ty where
   coe := Ty.from_action
 
 @[simp]
-def Ty.rmap (r : Ren) : Ty -> Ty
-| t#x => t#(r x)
+def Ty.rmap (r : Ren Ty) : Ty -> Ty
+| t#x => t#(r.act x)
 | gt#x => gt#x
 | A -:> B => rmap r A -:> rmap r B
 | ∀[K] P => ∀[K] rmap (r.lift) P
 | app f a => rmap r f • rmap r a
 | A ~[K]~ B => rmap r A ~[K]~ rmap r B
 
-instance : RenMap Ty where
+instance : RenMap Ty Ty where
   rmap := Ty.rmap
 
 @[simp]
-theorem Ty.ren_var : (t#x)⟨r⟩ = t#(r x) := by
+theorem Ty.ren_var {r : Ren Ty} : (t#x)⟨r⟩ = t#(r.act x) := by
   simp [RenMap.rmap]
 
 @[simp]
-theorem Ty.ren_global : (gt#x)⟨r⟩ = gt#x := by
+theorem Ty.ren_global {r : Ren Ty} : (gt#x)⟨r⟩ = gt#x := by
   simp [RenMap.rmap]
 
 @[simp]
-theorem Ty.ren_arr {A B : Ty} : (A -:> B)⟨r⟩ = A⟨r⟩ -:> B⟨r⟩ := by
+theorem Ty.ren_arr {A B : Ty} {r : Ren Ty} : (A -:> B)⟨r⟩ = A⟨r⟩ -:> B⟨r⟩ := by
   simp [RenMap.rmap]
 
 @[simp]
-theorem Ty.ren_all : (∀[K] P)⟨r⟩ = ∀[K] P⟨r.lift⟩ := by
+theorem Ty.ren_all {r : Ren Ty} : (∀[K] P)⟨r⟩ = ∀[K] P⟨r.lift⟩ := by
   simp [RenMap.rmap]
 
 @[simp]
-theorem Ty.ren_app : (f • a)⟨r⟩ = f⟨r⟩ • a⟨r⟩ := by
+theorem Ty.ren_app {r : Ren Ty} : (f • a)⟨r⟩ = f⟨r⟩ • a⟨r⟩ := by
   simp [RenMap.rmap]
 
 @[simp]
-theorem Ty.ren_eq : (A ~[K]~ B)⟨r⟩ = A⟨r⟩ ~[K]~ B⟨r⟩ := by
+theorem Ty.ren_eq {r : Ren Ty} : (A ~[K]~ B)⟨r⟩ = A⟨r⟩ ~[K]~ B⟨r⟩ := by
   simp [RenMap.rmap]
 
-instance : RenMapId Ty where
+instance : RenMapId Ty Ty where
   apply_id := by subst_solve_id
 
-instance : RenMapCompose Ty where
+instance : RenMapCompose Ty Ty where
   apply_compose := by subst_solve_compose
 
 @[simp]
 def Ty.smap (σ : Subst Ty) : Ty -> Ty
-| t#x => σ x
+| t#x => σ.act x
 | gt#x => gt#x
 | A -:> B => smap σ A -:> smap σ B
 | ∀[K] P => ∀[K] smap σ.lift P
@@ -83,42 +84,50 @@ instance : SubstMap Ty Ty where
   smap := Ty.smap
 
 @[simp]
-theorem Ty.subst_var : (t#x)[σ:Ty] = σ x := by
+theorem Ty.subst_var {σ : Subst Ty} : (t#x)[σ] = σ.act x := by
   simp [SubstMap.smap]
 
 @[simp]
-theorem Ty.subst_global : (gt#x)[σ:Ty] = gt#x := by
+theorem Ty.subst_global {σ : Subst Ty} : (gt#x)[σ] = gt#x := by
   simp [SubstMap.smap]
 
 @[simp]
-theorem Ty.subst_arr {A B : Ty} : (A -:> B)[σ:Ty] = A[σ:_] -:> B[σ:_] := by
+theorem Ty.subst_arr {σ : Subst Ty} {A B : Ty} : (A -:> B)[σ] = A[σ] -:> B[σ] := by
   simp [SubstMap.smap]
 
 @[simp]
-theorem Ty.subst_all : (∀[K] P)[σ:Ty] = ∀[K] P[σ.lift:_] := by
+theorem Ty.subst_all {σ : Subst Ty} : (∀[K] P)[σ] = ∀[K] P[σ.lift] := by
   simp [SubstMap.smap]
 
 @[simp]
-theorem Ty.subst_app : (f • a)[σ:Ty] = f[σ:_] • a[σ:_] := by
+theorem Ty.subst_app {σ : Subst Ty} : (f • a)[σ] = f[σ] • a[σ] := by
   simp [SubstMap.smap]
 
 @[simp]
-theorem Ty.subst_eq : (A ~[K]~ B)[σ:Ty] = A[σ:_] ~[K]~ B[σ:_] := by
+theorem Ty.subst_eq {σ : Subst Ty} : (A ~[K]~ B)[σ] = A[σ] ~[K]~ B[σ] := by
   simp [SubstMap.smap]
 
 @[simp]
-theorem Ty.from_action_compose {x} {σ τ : Subst Ty}
-  : (from_action (σ x))[τ] = from_action ((σ ∘ τ) x)
+theorem Ty.from_action_compose {x : Nat} {σ τ : Subst Ty}
+  : (from_action (σ.act x))[τ] = from_action ((σ ∘ τ).act x)
 := by
   simp [Ty.from_action, Subst.compose]
-  generalize zdef : σ x = z
+  generalize zdef : σ.act x = z
   cases z <;> simp [Ty.from_action]
+
+@[simp]
+theorem Ty.from_action_compose_ren {x : Nat} {σ : Subst Ty} {r : Ren Ty}
+  : (from_action (σ.act x))⟨r⟩ = from_action ((σ ∘ r).act x)
+:= by
+  simp [Ty.from_action]
+  generalize zdef : σ.act x = z
+  cases z <;> simp
 
 instance : SubstMapId Ty Ty where
   apply_id := by subst_solve_id
 
-instance : SubstMapStable Ty where
-  apply_stable := by subst_solve_stable
+-- instance : SubstMapStable Ty Ty where
+--   apply_stable := by subst_solve_stable
 
 instance : SubstMapRenComposeLeft Ty Ty where
   apply_ren_compose_left := by subst_solve_compose
@@ -130,88 +139,106 @@ instance : SubstMapCompose Ty Ty where
   apply_compose := by subst_solve_compose
 
 @[simp]
-def SpineTy.rmap (r : Ren) : SpineTy -> SpineTy
-| ⟨m, Ks, n, Ts, R⟩ =>
-  ⟨m, Ks, n, Vec.map (·[r.lift m]) Ts, R[r.lift m]⟩
+def SpineTy.rmap (r : Ren Ty) : SpineTy -> SpineTy
+| ⟨m1, Ks1, m2, Ks2, n, Ts, R⟩ =>
+  ⟨m1, Ks1, m2, Ks2, n, Vec.map (·⟨r.lift (m1 + m2)⟩) Ts, R⟨r.lift (m1 + m2)⟩⟩
 
-instance : RenMap SpineTy where
+instance : RenMap SpineTy Ty where
   rmap := SpineTy.rmap
 
 @[simp]
+theorem SpineTy.rmap_eq {r : Ren Ty}
+  : (⟨m1, Ks1, m2, Ks2, n, Ts, R⟩ : SpineTy)⟨r⟩
+    = ⟨m1, Ks1, m2, Ks2, n, Ts⟨r.lift (m1 + m2)⟩, R⟨r.lift (m1 + m2)⟩⟩
+:= by
+  simp [RenMap.rmap]
+  induction Ts <;> simp [Vec.rmap, *, RenMap.rmap]
+
+@[simp]
 def SpineTy.smap (σ : Subst Ty) : SpineTy -> SpineTy
-| ⟨m, Ks, n, Ts, R⟩ =>
-  ⟨m, Ks, n, Vec.map (·[σ.lift m]) Ts, R[σ.lift m]⟩
+| ⟨m1, Ks1, m2, Ks2, n, Ts, R⟩ =>
+  ⟨m1, Ks1, m2, Ks2, n, Vec.map (·[σ.lift (m1 + m2)]) Ts, R[σ.lift (m1 + m2)]⟩
 
 instance : SubstMap SpineTy Ty where
   smap := SpineTy.smap
 
 @[simp]
-theorem SpineTy.smap_eq : (⟨m, Ks, n, Ts, R⟩ : SpineTy)[σ:Ty] = ⟨m, Ks, n, Ts[σ.lift m:_], R[σ.lift m:_]⟩ := by
+theorem SpineTy.smap_eq {σ : Subst Ty}
+  : (⟨m1, Ks1, m2, Ks2, n, Ts, R⟩ : SpineTy)[σ]
+    = ⟨m1, Ks1, m2, Ks2, n, Ts[σ.lift (m1 + m2)], R[σ.lift (m1 + m2)]⟩
+:= by
   simp [SubstMap.smap]
   induction Ts <;> simp [Vec.smap, *, SubstMap.smap]
 
 instance : SubstMapId SpineTy Ty where
-  apply_id := by intro t; rcases t with ⟨m, Ks, n, Ts, R⟩; simp
+  apply_id := by intro t; rcases t with ⟨m1, Ks1, m2, Ks2, n, Ts, R⟩; simp
 
 instance : SubstMapRenComposeLeft SpineTy Ty where
-  apply_ren_compose_left := by intro t; rcases t with ⟨m, Ks, n, Ts, R⟩; simp
+  apply_ren_compose_left := by
+    intro t; rcases t with ⟨m1, Ks1, m2, Ks2, n, Ts, R⟩
+    simp [-Subst.rewrite_lift_k_ren, -Subst.rewrite_lift_k]
 
 instance : SubstMapRenComposeRight SpineTy Ty where
-  apply_ren_compose_right := by intro t; rcases t with ⟨m, Ks, n, Ts, R⟩; simp
+  apply_ren_compose_right := by
+    intro t; rcases t with ⟨m1, Ks1, m2, Ks2, n, Ts, R⟩
+    simp [-Subst.rewrite_lift_k_ren, -Subst.rewrite_lift_k]
 
 instance : SubstMapCompose SpineTy Ty where
-  apply_compose := by intro t; rcases t with ⟨m, Ks, n, Ts, R⟩; simp
+  apply_compose := by
+    intro t; rcases t with ⟨m1, Ks1, m2, Ks2, n, Ts, R⟩
+    simp [-Subst.rewrite_lift_k_ren, -Subst.rewrite_lift_k]
 
-theorem Ty.smap_promote : Ty.smap σ A = A[σ:Ty] := by simp [SubstMap.smap]
+theorem Ty.smap_promote : Ty.smap σ A = A[σ] := by simp [SubstMap.smap]
 
-theorem Ty.rename_preserves_var_shape {r : Ren} : t#x = T[r] -> ∃ y,  (T = t#y ∧ x = r y) := by
-  intro h
-  induction T <;> simp at *
-  case var => simp [Ren.to] at h; assumption
+-- theorem Ty.rename_preserves_var_shape {r : Ren Ty} : t#x = T⟨r⟩ -> ∃ y,  (T = t#y ∧ x = r.act y) := by
+--   sorry
+--   -- intro h
+--   -- induction T <;> simp at *
+--   -- case var => simp [Ren.to] at h; assumption
 
-theorem Ty.rename_preserves_global_shape {r : Ren} : gt#x = T[r] -> T = gt#x := by
-  intro h
-  induction T <;> simp at *
-  case var => simp [Ren.to] at h
-  case global => symm at h; assumption
+-- theorem Ty.rename_preserves_global_shape {r : Ren} : gt#x = T[r] -> T = gt#x := by
+--   intro h
+--   induction T <;> simp at *
+--   case var => simp [Ren.to] at h
+--   case global => symm at h; assumption
 
-theorem Ty.rename_preserves_arrow_shape {A B : Ty}{r : Ren} : A -:> B = T[r] ->
-  (∃ A' B' : Ty, (T = A' -:> B') ∧  A = A'[r] ∧ B = B'[r])
-:= by
-  intro h
-  induction T <;> simp at *
-  case var => simp [Ren.to] at h
-  case arrow a1 a2 _ _ => exists a1; exists a2
+-- theorem Ty.rename_preserves_arrow_shape {A B : Ty}{r : Ren} : A -:> B = T[r] ->
+--   (∃ A' B' : Ty, (T = A' -:> B') ∧  A = A'[r] ∧ B = B'[r])
+-- := by
+--   intro h
+--   induction T <;> simp at *
+--   case var => simp [Ren.to] at h
+--   case arrow a1 a2 _ _ => exists a1; exists a2
 
-theorem Ty.rename_preserves_eq_shape {A B : Ty}{r : Ren} : (A ~[K]~ B) = T[r] ->
-  (∃ A' B' : Ty, (T = A' ~[K]~ B') ∧  A = A'[r] ∧ B = B'[r])
-:= by
-  intro h
-  induction T generalizing K  <;> simp at *
-  case var => simp [Ren.to] at h
-  case eq a1 a2 _ _  =>
-    cases h.1; cases h.2.1; cases h.2.2; clear h
-    exists a1; exists a2
+-- theorem Ty.rename_preserves_eq_shape {A B : Ty}{r : Ren} : (A ~[K]~ B) = T[r] ->
+--   (∃ A' B' : Ty, (T = A' ~[K]~ B') ∧  A = A'[r] ∧ B = B'[r])
+-- := by
+--   intro h
+--   induction T generalizing K  <;> simp at *
+--   case var => simp [Ren.to] at h
+--   case eq a1 a2 _ _  =>
+--     cases h.1; cases h.2.1; cases h.2.2; clear h
+--     exists a1; exists a2
 
-theorem Ty.rename_preserves_app_shape {A B : Ty}{r : Ren} : (A • B) = T[r] ->
-  (∃ A' B' : Ty, (T = A' • B') ∧  A = A'[r] ∧ B = B'[r])
-:= by
-  intro h
-  induction T <;> simp at *
-  case var => simp [Ren.to] at h
-  case app a1 a2 _ _  =>
-    cases h.1; cases h.2; clear h
-    exists a1; exists a2
+-- theorem Ty.rename_preserves_app_shape {A B : Ty}{r : Ren} : (A • B) = T[r] ->
+--   (∃ A' B' : Ty, (T = A' • B') ∧  A = A'[r] ∧ B = B'[r])
+-- := by
+--   intro h
+--   induction T <;> simp at *
+--   case var => simp [Ren.to] at h
+--   case app a1 a2 _ _  =>
+--     cases h.1; cases h.2; clear h
+--     exists a1; exists a2
 
 
-theorem Ty.rename_preserves_all_shape {P : Ty}{r : Ren} : (∀[K] P) = T[r] ->
-  (∃ P' : Ty, (T = ∀[K]P') ∧  P = P'[re 0::↑r ∘ +1:Ty])
-:= by
-  intro h
-  induction T generalizing K P <;> simp at *
-  case var => simp [Ren.to] at h
-  case all a ih =>
-    cases h.1; cases h.2; clear h
-    exists a;
+-- theorem Ty.rename_preserves_all_shape {P : Ty}{r : Ren} : (∀[K] P) = T[r] ->
+--   (∃ P' : Ty, (T = ∀[K]P') ∧  P = P'[re 0::↑r ∘ +1:Ty])
+-- := by
+--   intro h
+--   induction T generalizing K P <;> simp at *
+--   case var => simp [Ren.to] at h
+--   case all a ih =>
+--     cases h.1; cases h.2; clear h
+--     exists a;
 
 end Core
